add trace to solved predicate

lambda.v
@@ -2,15 +2,33 @@ Require Import List ssreflect.
 Import ListNotations.
 
 Inductive term : Type :=
-  (* tm n x [t1; ...; tk] is the term
+  (* tm n x [tk; ...; t1] is the term
      \x1...\xn. x t1 ... tk
      where x is the de Bruijn index of a bound variable.
      If the variable is out of bounds, then it is a constant *)
   | tm : nat -> nat -> list term -> term.
 
-Inductive lookup : Type :=
-  | lk : list (term * lookup) -> lookup.
+(* a path is a list of indices to traverse a term *)
 
+(* compute the subterm of t at path p *)
+Fixpoint subterm (t : term) (p : list nat) : option term :=
+  match t, p with
+  | tm n x ts, [] => Some (tm n x ts)
+  | tm n x ts, i :: p =>
+    match nth_error ts i with
+    | Some ti => subterm ti p
+    | None => None
+    end
+  end.
+
+Inductive rose_tree (A : Type) : Type :=
+  | node : A -> list (rose_tree A) -> rose_tree A.
+
+Arguments node {A}.
+
+Inductive lookup : Type :=
+  | lk : list ((nat * list nat) * lookup) -> lookup.
+(*
 (* 
   (x, [t1; ...; tk], l, t) is the state
   where x is the de Bruijn index of head symbol
@@ -19,49 +37,51 @@ Inductive lookup : Type :=
   t is the current right-hand side term
 *)
 Notation state := (nat * list term * list (term * lookup) * term)%type.
-
-Definition add_lk (l : list (term * lookup)) (t : term) :=
-  (t, lk l).
+*)
+Definition add_lk (i : nat) (p : list nat) (theta : list ((nat * list nat) * lookup)) (j : nat) :=
+  ((i, p ++ [j]), lk theta).
 
 Arguments add_lk /.
 
 (* for now / for simplicity let us consider rhs which does not contain abstraction
   e.g. f (\x.x) is not allowed as right-hand side
 *)
-(* solved theta x ts z rs means that
-   x applied to the terms ts with free variables substituted according to theta
-   reduces to z applied to rs
+
+(*
+  solved TS i p theta game_tree r
+    TS = [t, t1, ..., tk] where t is the solution and t1, ..., tk are arguments
+    i is the term index in TS
+    p is the path to the subterm in the particular term
+    theta is the lookup table for free variables
+    game_tree are positions ((i', p'), theta') in the game
+    r is the rhs term (no abstractions)
+  means that the game starting at position ((i, p), theta) with the rhs r is solved
 *)
-Inductive solved : list (term * lookup) -> nat -> list term -> nat -> list term -> Prop :=
-  | solved_var (x y : nat) (m : nat) (ts us : list term) (theta theta' : list (term * lookup))
-    (z : nat) (rs : list term) :
-    nth_error theta x = Some (tm m y us, lk theta') ->
-    solved ((map (add_lk theta) (rev ts)) ++ theta') y us z rs ->
-    solved theta x ts z rs
-  | solved_const (x : nat) (ts us : list term) (theta : list (term * lookup)) :
-    Forall2 (fun t u => match t, u with tm nt _ _, tm nu _ _ => nt = 0 /\ nu = 0 end) ts us ->
-    (forall xt tts xu uts, In (tm 0 xt tts, tm 0 xu uts) (combine ts us) ->
-      solved theta xt tts xu uts) ->
-    solved theta (x + length theta) ts x us.
 
-(* alternative characterization *)
-Lemma solved_const' (x : nat) (ts us : list term) (theta : list (term * lookup)) :
-  Forall2 (fun t u => match t, u with tm nt xt tts, tm nu xu uts => nt = 0 /\ nu = 0 /\ solved theta xt tts xu uts end) ts us ->
-  solved theta (x + length theta) ts x us.
-Proof.
-  move=> H. apply: solved_const.
-  - apply: Forall2_impl H.
-    by move=> [] ??? [] ??? [->] [->].
-  - elim: H; first done.
-    move=> > H' ? IH > /= [].
-    + move=> [??]. subst. tauto.
-    + by apply: IH.
-Qed.
+Inductive solved (TS : list term) (i : nat) (p : list nat) (theta : list ((nat * list nat) * lookup)) :
+  rose_tree ((nat * list nat) * list ((nat * list nat) * lookup)) ->
+  rose_tree nat -> Prop :=
+    | solved_var t n x ts j q theta' r g :
+      nth_error TS i = Some t ->
+      subterm t p = Some (tm n x ts) ->
+      nth_error theta x = Some ((j, q), lk theta') ->
+      solved TS j q ((map (add_lk i p theta) (seq 0 (length ts))) ++ theta') g r ->
+      solved TS i p theta (node ((i, p), theta) [g]) r
+    | solved_const t gs n x ts rs :
+      nth_error TS i = Some t ->
+      subterm t p = Some (tm n (x + length theta) ts) ->
+      length ts = length rs ->
+      Forall2 (fun _ t => match t with tm nt _ _ => nt = 0 end) gs ts ->
+      (forall g j r, In (g, (j, r)) (combine gs (combine (seq 0 (length rs)) rs)) ->
+        solved TS i (p ++ [j]) theta g r) ->
+      solved TS i p theta (node ((i, p), theta) gs) (node x rs).
 
-(* t ts = u *)
-Definition solved_start t (ts : list term) u :=
-  match t, u with
-  | tm n x us, tm m z rs => length ts = n /\ m = 0 /\ solved (map (add_lk []) (rev ts)) x us z rs
+(* t ts = r *)
+Definition solved_start g t (ts : list term) (r : rose_tree nat) :=
+  match t with
+  | tm n x us =>
+    length ts = n /\
+    solved (t :: ts) 0 [] (map (fun j => ((S j, []), lk [])) (rev (seq 0 (length ts)))) g r
   end.
 
 (*
@@ -73,14 +93,22 @@ Definition solved_start t (ts : list term) u :=
 Definition ex1_0 := tm 1 0 [].
 (* a *)
 Definition ex1_1 := tm 0 0 [].
+(* a as applicative term *)
+Definition ex1_rhs := node 0 [].
 
-Lemma solved_ex1 : solved_start ex1_0 [ex1_1] ex1_1.
+Lemma solved_ex1 : exists g, solved_start g ex1_0 [ex1_1] ex1_rhs.
 Proof.
-  cbn. split; [|split]; [reflexivity..|].
+  eexists.
+  cbn. split; [reflexivity|].
   apply: solved_var.
   - cbn. reflexivity.
-  - cbn. apply: (solved_const 0).
-    + constructor.
+  - cbn. reflexivity.
+  - cbn. reflexivity.
+  - cbn. apply: solved_const.
+    + cbn. reflexivity.
+    + cbn. reflexivity.
+    + cbn. reflexivity.
+    + cbn. constructor.
     + done.
 Qed.
 
@@ -92,47 +120,49 @@ Qed.
 *)
 
 Definition main_solution :=
-  tm 2 0 [tm 2 3 [tm 0 1 []; tm 2 5 [tm 0 8 []; tm 2 4 [tm 0 3 []; tm 0 3 []]]]].
+  tm 2 0 [tm 2 3 [tm 2 5 [tm 2 4 [tm 0 3 []; tm 0 3 []]; tm 0 8 []]; tm 0 1 []]].
 
 Definition arg1 :=
   tm 2 0 [tm 0 1 []; tm 0 1 []].
 
 Definition arg2 :=
-  tm 1 0 [tm 0 0 [tm 0 1 []; tm 2 1 []]; tm 2 4 [tm 0 0 []]].
+  tm 1 0 [tm 2 4 [tm 0 0 []]; tm 0 0 [tm 2 1 []; tm 0 1 []]].
 
 (* g a *)
 Definition result :=
-  tm 0 1 [tm 0 0 []].
+  node 1 [node 0 []].
 
-Lemma solved_Stirling : solved_start main_solution [arg1; arg2] result.
+Lemma solved_Stirling : exists g, solved_start g main_solution [arg1; arg2] result.
 Proof.
-  unfold main_solution, arg1, arg2, result.
-  cbn. split; [|split]; [reflexivity..|].
-  apply: solved_var. { reflexivity. }
-  apply: solved_var. { reflexivity. }
-  apply: solved_var. { reflexivity. }
-  apply: solved_var. { reflexivity. }
-  apply: solved_var. { reflexivity. }
-  apply: solved_var. { reflexivity. }
-  apply: solved_var. { reflexivity. }
+  unfold result.
+  eexists.
+  cbn. split; [reflexivity|].
+  apply: solved_var; [reflexivity..|].
+  rewrite [length _]/=. apply: solved_var; [reflexivity..|].
+  rewrite [length _]/=. apply: solved_var; [reflexivity..|].
+  rewrite [length _]/=. apply: solved_var; [reflexivity..|].
+  rewrite [length _]/=. apply: solved_var; [reflexivity..|].
+  rewrite [length _]/=. apply: solved_var; [reflexivity..|].
+  rewrite [length _]/=. apply: solved_var; [reflexivity..|].
 
-  apply: (solved_const' 1). constructor; last done.
-  split; [done|split; [done|]].
+  rewrite [length _]/=. apply: solved_const; [repeat constructor..|].
+  move=> > [|]; last done.
+  move=> [*]. subst.
+  apply: solved_var; [reflexivity..|].
+  rewrite [length _]/=. apply: solved_var; [reflexivity..|].
+  rewrite [length _]/=. apply: solved_var; [reflexivity..|].
+  rewrite [length _]/=. apply: solved_var; [reflexivity..|].
+  rewrite [length _]/=. apply: solved_var; [reflexivity..|].
+  rewrite [length _]/=. apply: solved_var; [reflexivity..|].
+  rewrite [length _]/=. apply: solved_var; [reflexivity..|].
+  rewrite [length _]/=. apply: solved_var; [reflexivity..|].
+  rewrite [length _]/=. apply: solved_var; [reflexivity..|].
+  rewrite [length _]/=. apply: solved_var; [reflexivity..|].
+  rewrite [length _]/=. apply: solved_var; [reflexivity..|].
+  rewrite [length _]/=. apply: solved_var; [reflexivity..|].
+  rewrite [length _]/=. apply: solved_var; [reflexivity..|].
+  rewrite [length _]/=. apply: solved_var; [reflexivity..|].
 
-  apply: solved_var. { reflexivity. }
-  apply: solved_var. { reflexivity. }
-  apply: solved_var. { reflexivity. }
-  apply: solved_var. { reflexivity. }
-  apply: solved_var. { reflexivity. }
-  apply: solved_var. { reflexivity. }
-  apply: solved_var. { reflexivity. }
-  apply: solved_var. { reflexivity. }
-  apply: solved_var. { reflexivity. }
-  apply: solved_var. { reflexivity. }
-  apply: solved_var. { reflexivity. }
-  apply: solved_var. { reflexivity. }
-  apply: solved_var. { reflexivity. }
-  apply: solved_var. { reflexivity. }
-
-  apply: (solved_const' 0). constructor.
+  rewrite [length _]/=. apply: solved_const; [repeat constructor..|].
+  done.
 Qed.
